theories/Prelude/X.v
@@ -149,3 +149,255 @@ Proof.
     contradiction NOT_IN. erewrite INJ with (a := a) (b := b); simpl; eauto with *.
   - eapply IH. intros a1 b1 a1_in b1_in H_eq.  exact (INJ a1 b1 (or_intror a1_in) (or_intror b1_in) H_eq).
 Qed.
+
+Module SN.
+
+Section Strong_Normalisation.
+
+Context {A : Type}.
+
+Inductive sn (R : A -> A -> Prop) (x : A) : Prop :=
+  | sn_intro
+    (sn_inv : forall x' : A, R x x' -> sn R x').
+
+Context {R : A -> A -> Prop}.
+
+Definition sn_inv (x : A) (H_sn : sn R x) : forall x' : A, R x x' -> sn R x' :=
+  match H_sn with
+  | @sn_intro _ _ sn_inv => sn_inv
+  end.
+
+Fixpoint sn_guard {x : A} (n : nat) (H_sn : sn R x) {struct n} : sn R x :=
+  match n with
+  | O => H_sn
+  | S n' => sn_intro R x (fun x' : A => fun H_R : R x x' => sn_guard n' (sn_inv x H_sn x' H_R))
+  end.
+
+End Strong_Normalisation.
+
+Strategy 100 [sn_guard].
+
+Section Strict_Progress_on_Prosets.
+
+Context {A : Type} {PROSET : isProset A}.
+
+Inductive betaProgressive (x : A) (x' : A) : Prop :=
+  | betaProgressive_intro
+    (LE : x =< x')
+    (NE : ~ (x == x')).
+
+Theorem finite_upper_cone_implies_sn (x0 : A)
+  (finite_upper_cone : exists cone : list A, forall x : A, x0 =< x -> L.In x cone)
+  : sn betaProgressive x0.
+Proof.
+  destruct finite_upper_cone as [cone IN].
+  enough (INV : forall bound : nat, forall cone : list A, forall x : A, length cone <= bound -> (forall y : A, x =< y -> L.In y cone) -> sn betaProgressive x).
+  { eapply INV with (bound := length cone) (cone := cone); eauto. }
+  induction bound as [ | bound IH]; intros cone' x LENGTH UPPER.
+  - destruct cone' as [ | a cone']; simpl in LENGTH.
+    + exfalso. eapply UPPER. reflexivity.
+    + lia.
+  - pose proof (UPPER x (leProp_refl x)) as IN_X.
+    apply L.in_split in IN_X. destruct IN_X as (prefix & suffix & CONE_EQ).
+    subst cone'. econs. intros x' [LE NE].
+    eapply IH with (cone := prefix ++ suffix).
+    + rewrite !length_app in LENGTH |- *. simpl in LENGTH. lia.
+    + intros y LE'.
+      pose proof (UPPER y (leProp_trans x x' y LE LE')) as IN_Y.
+      rewrite L.in_app_iff in IN_Y. simpl in IN_Y.
+      rewrite L.in_app_iff. destruct IN_Y as [IN_Y | [Y_EQ | IN_Y]]; eauto.
+      subst y. contradiction NE. eapply leProp_antisymmetry; eauto.
+Qed.
+
+Corollary finite_domain_guarantees_sn
+  (FINITE : exists enum : list A, forall x : A, L.In x enum)
+  : forall x0 : A, sn betaProgressive x0.
+Proof.
+  destruct FINITE as [enum IN]. i.
+  eapply finite_upper_cone_implies_sn; ss!.
+Qed.
+
+Section Progressive_Fixed_Point_Iteration.
+
+Context {eqProp_dec : forall x : A, forall x' : A, B.Decision (x == x')}.
+
+Variable step : A -> A.
+
+Hypothesis step_isProgressive : forall x : A, x =< step x.
+
+Fixpoint prog_iter (x : A) (sn_x : sn betaProgressive x) {struct sn_x} : A :=
+  let x' : A := step x in
+  match B.decide (x == x') with
+  | left H_EQ => x
+  | right H_NE => prog_iter x' (sn_inv x sn_x x' (betaProgressive_intro x x' (step_isProgressive x) H_NE))
+  end.
+
+Fixpoint prog_iter_pirrel (x : A) (H_sn : sn betaProgressive x) (H_sn' : sn betaProgressive x) {struct H_sn} : prog_iter x H_sn = prog_iter x H_sn'.
+Proof.
+  destruct H_sn as [H_sn_inv], H_sn' as [H_sn_inv']; simpl.
+  destruct (B.decide _) as [H_EQ | H_NE]; [reflexivity | eapply prog_iter_pirrel].
+Qed.
+
+Fixpoint prog_iter_isProgressive (x : A) (sn_x : sn betaProgressive x) {struct sn_x} : x =< prog_iter x sn_x.
+Proof.
+  destruct sn_x as [H_sn_inv]. simpl.
+  destruct (B.decide _) as [H_EQ | H_NE].
+  - reflexivity.
+  - etransitivity.
+    + eapply step_isProgressive.
+    + eapply prog_iter_isProgressive.
+Qed.
+
+Fixpoint prog_iter_isFixedpoint (x : A) (sn_x : sn betaProgressive x) {struct sn_x} : step (prog_iter x sn_x) == prog_iter x sn_x.
+Proof.
+ destruct sn_x as [H_sn_inv]. simpl.
+  destruct (B.decide _) as [H_EQ | H_NE].
+  - symmetry. exact H_EQ.
+  - eapply prog_iter_isFixedpoint.
+Qed.
+
+Hypothesis step_isMonotonic : isMonotonic1 step.
+
+Fixpoint prog_iter_le (x : A) (x' : A) (sn_x : sn betaProgressive x) (FIXEDPOINT : step x' == x') (LE : x =< x') {struct sn_x} : prog_iter x sn_x =< x'.
+Proof.
+  destruct sn_x as [H_sn_inv]; simpl.
+  destruct (B.decide _) as [H_EQ | H_NE].
+  - exact LE.
+  - eapply prog_iter_le.
+    + exact FIXEDPOINT.
+    + etransitivity.
+      * eapply step_isMonotonic. exact LE.
+      * eapply eqProp_implies_leProp. exact FIXEDPOINT.
+Qed.
+
+End Progressive_Fixed_Point_Iteration.
+
+End Strict_Progress_on_Prosets.
+
+Section STRONG_SEARCH.
+
+Fixpoint add' (n : nat) (m : nat) {struct n} : nat :=
+  match n with
+  | O => m
+  | S n' => add' n' (S m)
+  end.
+
+Context {State : Type} (isDone : nat -> State -> Prop) {isDone_dec : forall n : nat, forall s : State, B.Decision (isDone n s)}.
+
+Variable step : nat -> State -> State.
+
+Definition advance (n : nat) (s : State) : State :=
+  if B.decide (isDone n s) then s else step n s.
+
+Variable s0 : State.
+
+Fixpoint trace (n : nat) : State :=
+  match n with
+  | O => s0
+  | S n' => advance n' (trace n')
+  end.
+
+Let P (n : nat) : Prop :=
+  isDone n (trace n).
+
+Inductive search (n : nat) : nat -> Prop :=
+  | search_next
+    (NOT_P : ~ (P n))
+    : search n (S n).
+
+Fixpoint strong_search_go (n : nat) (s : State) (Hs : s = trace n) (sn_n : sn search n) {struct sn_n} : nat * State.
+Proof.
+  destruct (B.decide (isDone n s)) as [H_YES | H_NO].
+  - exact (n, s).
+  - set (s' := step n s).
+    assert (NOT_P : ~ (P n)).
+    { unfold P. rewrite <- Hs. exact H_NO. }
+    assert (Hs' : s' = trace (S n)).
+    { unfold s'. simpl. unfold advance.
+      destruct (B.decide _) as [H_YES' | H_NO'].
+      - contradiction H_NO. congruence.
+      - congruence.
+    }
+    exact (strong_search_go (S n) s' Hs' (sn_inv n sn_n (S n) (search_next n NOT_P))).
+Defined.
+
+Lemma add'_zero_r n
+  : add' n 0 = n.
+Proof.
+  enough (AUX : forall p, forall q, add' p q = p + q).
+  { rewrite AUX. lia. }
+  intros p. induction p as [ | p IH]; intros q; simpl.
+  - reflexivity.
+  - rewrite IH. lia.
+Qed.
+
+Lemma sn_search n k
+  (WITNESS : P (add' n k))
+  : sn search n.
+Proof.
+  revert n WITNESS. induction k as [ | k IH]; intros n WITNESS.
+  - constructor. intros n' SEARCH. destruct SEARCH as [NOT_P].
+    contradiction NOT_P. rewrite <- add'_zero_r. exact WITNESS.
+  - constructor. intros n' SEARCH. destruct SEARCH as [NOT_P].
+    eapply IH. simpl. exact WITNESS.
+Qed.
+
+Hypothesis eventually_stops : exists k : nat, P k.
+
+Corollary sn_search_0
+  : sn search 0.
+Proof.
+  destruct eventually_stops as [k WITNESS].
+  exact (sn_search O k WITNESS).
+Qed.
+
+Definition strong_search : nat * State :=
+  strong_search_go 0 s0 eq_refl sn_search_0.
+
+Fixpoint strong_search_go_pirrel (n : nat) (s : State) (Hs : s = trace n) (Hs' : s = trace n) (sn_n : sn search n) (sn_n' : sn search n) {struct sn_n} : strong_search_go n s Hs sn_n = strong_search_go n s Hs' sn_n'.
+Proof.
+  destruct sn_n as [H_sn_inv], sn_n' as [H_sn_inv']; simpl.
+  destruct (B.decide _) as [H_YES | H_NO].
+  - reflexivity.
+  - eapply strong_search_go_pirrel.
+Qed.
+
+Lemma strong_search_go_correct_from (n : nat) (s : State) (n' : nat) (s' : State)
+  (Hs : s = trace n)
+  (sn_n : sn search n)
+  (RESULT : (n', s') = strong_search_go n s Hs sn_n)
+  : trace n' = s' /\ isDone n' s' /\ (forall m : nat, n <= m -> m < n' -> ~ (isDone m (trace m))).
+Proof.
+  revert n s Hs sn_n n' s' RESULT. fix IH 4. intros n s Hs [H_sn_inv] n' s' RESULT. simpl in RESULT.
+  destruct (B.decide (isDone n s)) as [H_YES | H_NO].
+  - inversion RESULT; subst n' s'. split.
+    + symmetry. exact Hs.
+    + split; [exact H_YES | lia].
+  - find* (TRACE & DONE & FIRST) by IH.
+    split; [exact TRACE | split; [exact DONE | intros m N_LE_M M_LT]].
+    pose proof (Nat.eq_dec m n) as [EQ | NE].
+    + subst m. unfold P. rewrite <- Hs. exact H_NO.
+    + eapply FIRST; lia.
+Qed.
+
+Theorem strong_search_correct (n : nat) (s : State)
+  (H_strong_search : (n, s) = strong_search)
+  : trace n = s /\ isDone n s /\ (forall m : nat, m < n -> ~ (isDone m (trace m))).
+Proof.
+  find* (TRACE & DONE & FIRST) by strong_search_go_correct_from.
+  split; [exact TRACE | split; [exact DONE | intros m LT]].
+  eapply FIRST; lia.
+Qed.
+
+Definition strong_search_with_budget (budget : nat) : nat * State :=
+  strong_search_go 0 s0 eq_refl (sn_guard (S budget) sn_search_0).
+
+Theorem strong_search_with_budget_eq (budget : nat)
+  : strong_search_with_budget budget = strong_search.
+Proof.
+  eapply strong_search_go_pirrel.
+Qed.
+
+End STRONG_SEARCH.
+
+End SN.
